Tactics: exposing full check_equiv with both flags

ocaml/fstar-lib/FStar_Tactics_V2_Builtins.ml
@@ -142,7 +142,7 @@ type ('env, 'sc, 't, 'pats, 'bnds) match_complete_token = unit
 
 let is_non_informative           = from_tac_2 "B.refl_is_non_informative" B.refl_is_non_informative
 let check_subtyping              = from_tac_3 "B.refl_check_subtyping" B.refl_check_subtyping
-let check_equiv                  = from_tac_3 "B.refl_check_equiv" B.refl_check_equiv
+let t_check_equiv                = from_tac_5 "B.t_refl_check_equiv" B.t_refl_check_equiv
 let core_compute_term_type       = from_tac_2 "B.refl_core_compute_term_type" B.refl_core_compute_term_type
 let core_check_term              = from_tac_4 "B.refl_core_check_term" B.refl_core_check_term
 let core_check_term_at_type      = from_tac_3 "B.refl_core_check_term_at_type" B.refl_core_check_term_at_type
