src/tactics/FStar.Tactics.V2.Basic.fst
@@ -2268,7 +2268,7 @@ let refl_is_non_informative (g:env) (t:typ) : tac (option unit & issues) =
     return (None, [unexpected_uvars_issue (Env.get_range g)])
   )
 
-let refl_check_relation (smt_ok:bool) (unfolding_ok:bool) (g:env) (t0 t1:typ) (rel:relation)
+let refl_check_relation (rel:relation) (smt_ok:bool) (unfolding_ok:bool) (g:env) (t0 t1:typ)
   : tac (option unit * issues) =
 
   if no_uvars_in_g g &&
@@ -2301,10 +2301,9 @@ let refl_check_relation (smt_ok:bool) (unfolding_ok:bool) (g:env) (t0 t1:typ) (r
   )
 
 let refl_check_subtyping (g:env) (t0 t1:typ) : tac (option unit & issues) =
-  refl_check_relation true true g t0 t1 Subtyping
+  refl_check_relation Subtyping true true g t0 t1
 
-let refl_check_equiv (g:env) (t0 t1:typ) : tac (option unit & issues) =
-  refl_check_relation true true g t0 t1 Equality
+let t_refl_check_equiv = refl_check_relation Equality
 
 let to_must_tot (eff:Core.tot_or_ghost) : bool =
   match eff with
